eIris/proofmode/base.v
@@ -95,4 +95,4 @@ Proof.
   rewrite HP12 /=. *)
 End tactics.
 
-Ltac intros_anon := intros ?.
+(* Ltac intros_anon := intros ?. *)
